finish simplifying concretization

src/rocq/Handlers/Concretization.v
@@ -231,16 +231,7 @@ Module Type ConcretizationBase (LP : LLVMParams) (MP : MEMORY_PARAMS LP) (Byte :
 
   Parameter ptr_size : nat.
   Parameter endianess : Endianess.
-  Parameter concretize_uvalueM :
-    forall (M : Type -> Type) `{Monad M} (handler : dtyp -> M dvalue)
-      (ERR_M : Type -> Type) `{Monad ERR_M} `{RAISE_ERROR ERR_M} `{RAISE_UB ERR_M} `{RAISE_OOM ERR_M},
-      (forall A : Type, ERR_M A -> M A) -> uvalue -> M dvalue.
 
-  Parameter eval_select :
-    forall (M : Type -> Type) `{Monad M} (handler : dtyp -> M dvalue)
-      (ERR_M : Type -> Type) `{Monad ERR_M} `{RAISE_ERROR ERR_M} `{RAISE_UB ERR_M} `{RAISE_OOM ERR_M}
-      (lift_ue : forall A : Type, ERR_M A -> M A)
-      (cnd : dvalue) (v1 v2 : uvalue), M dvalue.
 
   Definition pre_concretized (acc : NMap (list (uvalue * dvalue))) (uv : uvalue) (sid : store_id) : option dvalue
     := vs <- NM.find sid acc;;
@@ -259,12 +250,19 @@ Module Type ConcretizationBase (LP : LLVMParams) (MP : MEMORY_PARAMS LP) (Byte :
        | None =>
            NM.add sid [(uv, dv)] acc
        end.
+
   (* Equations *)
-  Parameter concretize_uvalueM_equation :
-    forall (M : Type -> Type) {HM : Monad M} (undef_handler : dtyp -> M dvalue)
-      (ERR_M : Type -> Type) {HM_ERR : Monad ERR_M} {ERR : RAISE_ERROR ERR_M} {UB : RAISE_UB ERR_M}
-      {OOM : RAISE_OOM ERR_M} (lift_ue : forall A : Type, ERR_M A -> M A) (u : uvalue),
-      concretize_uvalueM M undef_handler ERR_M lift_ue u =
+  Fixpoint concretize_uvalueM 
+      (M : Type -> Type) `{HM : Monad M} (undef_handler : dtyp -> M dvalue)
+      (ERR_M : Type -> Type) `{HM_ERR : Monad ERR_M} `{ERR: RAISE_ERROR ERR_M} `{UP : RAISE_UB ERR_M} `{OOM : RAISE_OOM ERR_M}
+      (lift_ue : forall A : Type, ERR_M A -> M A) (u:uvalue) : M dvalue :=
+
+  
+  (* Parameter concretize_uvalueM_equation : *)
+  (*   forall (M : Type -> Type) {HM : Monad M} (undef_handler : dtyp -> M dvalue) *)
+  (*     (ERR_M : Type -> Type) {HM_ERR : Monad ERR_M} {ERR : RAISE_ERROR ERR_M} {UB : RAISE_UB ERR_M} *)
+  (*     {OOM : RAISE_OOM ERR_M} (lift_ue : forall A : Type, ERR_M A -> M A) (u : uvalue), *)
+  (*     concretize_uvalueM M undef_handler ERR_M lift_ue u = *)
         let
           eval_select
             (cnd : dvalue) (v1 v2 : uvalue) : M dvalue
@@ -484,12 +482,11 @@ Module Type ConcretizationBase (LP : LLVMParams) (MP : MEMORY_PARAMS LP) (Byte :
         | _ => lift_ue _ (raise_error ("concretize_uvalueM: Attempting to convert a partially non-reduced uvalue to dvalue. Should not happen: " ++ uvalue_constructor_string u))
         end.
 
-      Parameter eval_select_equation :
-        forall (M : Type -> Type) {HM : Monad M} (undef_handler : dtyp -> M dvalue)
-          (ERR_M : Type -> Type) {HM_ERR : Monad ERR_M} {ERR : RAISE_ERROR ERR_M} {UB : RAISE_UB ERR_M}
-          {OOM : RAISE_OOM ERR_M} (lift_ue : forall A : Type, ERR_M A -> M A)
-          (cnd : dvalue) (v1 v2 : uvalue),
-          eval_select M undef_handler ERR_M lift_ue cnd v1 v2 =
+    Definition eval_select
+      (M : Type -> Type) `{Monad M} (undef_handler : dtyp -> M dvalue)
+      (ERR_M : Type -> Type) `{Monad ERR_M} `{RAISE_ERROR ERR_M} `{RAISE_UB ERR_M} `{RAISE_OOM ERR_M}
+      (lift_ue : forall A : Type, ERR_M A -> M A)
+      (cnd : dvalue) (v1 v2 : uvalue) : M dvalue :=
             match cnd with
             | DVALUE_Poison t =>
                 (* TODO: Should be the type of the result of the select... *)
@@ -630,7 +627,7 @@ Module Type Concretization (LP : LLVMParams) (MP : MEMORY_PARAMS LP) (Byte : Byt
     intros dt dv DVT H.
     rewrite concretize_equation.
     unfold concretize_u.
-    rewrite concretize_uvalueM_equation.
+    unfold concretize_uvalueM.
     cbn; auto.
   Qed.
 
@@ -645,7 +642,7 @@ Module Type Concretization (LP : LLVMParams) (MP : MEMORY_PARAMS LP) (Byte : Byt
     intros iop uv1 e1 uv2 e2 C1 C2.
     unfold concretize_u in *.
 
-    rewrite concretize_uvalueM_equation.
+    unfold concretize_uvalueM.
     red.
 
     unfold bind.
@@ -707,179 +704,11 @@ Module MakeBase (LP : LLVMParams) (MP : MEMORY_PARAMS LP) (Byte : ByteModule LP 
   Open Scope list.
 
   Export Byte.
+  Include ConcretizationBase LP MP Byte
+    with Definition ptr_size := (8%nat)
+    with Definition endianess := ENDIAN_LITTLE.
 
-  Module MemHelpers := MemoryHelpers LP MP Byte.
-  Import MemHelpers.
-
-  Definition eval_icmp {M} `{Monad M} `{RAISE_ERROR M} (samesign:bool) (icmp : icmp) (v1 v2 : dvalue) : M dvalue.
-    refine
-      (match v1, v2 with
-       | @DVALUE_I sz1 i1, @DVALUE_I sz2 i2 =>
-           _
-       | DVALUE_IPTR i1, DVALUE_IPTR i2 => eval_int_icmp samesign icmp i1 i2
-       | DVALUE_Poison t1, DVALUE_Poison t2 => ret (DVALUE_Poison t1)
-       | DVALUE_Poison t, _ => if is_DVALUE_IX v2 then ret (DVALUE_Poison t) else raise_error "ill_typed-iop"
-       | _, DVALUE_Poison t => if is_DVALUE_IX v1 then ret (DVALUE_Poison t) else raise_error "ill_typed-iop"
-       | DVALUE_Addr a1, DVALUE_Addr a2 =>
-           let i1 := ptr_to_int a1 in
-           let i2 := ptr_to_int a2 in
-           eval_int_icmp false icmp i1 i2
-       | _, _ => raise_error ("ill_typed-icmp: " ++ show_dvalue v1 ++ ", " ++ show_dvalue v2)
-       end).
-    destruct (Pos.eq_dec sz1 sz2); subst.
-    - exact (eval_int_icmp samesign icmp i1 i2).
-    - exact (raise_error ("ill_typed-icmp: " ++ show_dvalue v1 ++ ", " ++ show_dvalue v2)).
-  Defined.
-  Arguments eval_icmp _ _ _ _ : simpl nomatch.
-
-  Section CONVERSIONS.
-
-    (** ** Typed conversion
-        Performs a dynamic conversion of a [dvalue] of type [t1] to one of type [t2].
-        For instance, convert an integer over 8 bits to one over 1 bit by truncation.
-
-        The conversion function is not pure, i.e. in particular cannot live in [DynamicValues.v]
-        as would be natural, due to the [Int2Ptr] and [Ptr2Int] cases. At those types, the conversion
-        needs to cast between integers and pointers, which depends on the memory model.
-     *)
-
-    (* Note: Inferring the subevent instance takes a small but non-trivial amount of time,
-       and has to be done here hundreds and hundreds of times due to the brutal pattern matching on
-       several values. Factoring the inference upfront is therefore necessary.
-     *)
-
-    (* A trick avoiding proofs that involve thousands of cases: we split the conversion into
-      the composition of a huge case analysis that builds a value of [conv_case], and a function
-      with only four cases to actually build the tree.
-     *)
-    Definition get_conv_case (conv : conversion_type) (t1:dtyp) (x:dvalue) (t2:dtyp) : conv_case :=
-      match conv with
-      | Trunc nuw nsb => (* TODO: handle the nuw and nsb flags *)
-          match t1, x, t2 with
-          | DTYPE_I sz_t, @DVALUE_I sz_from i1, DTYPE_I sz_to =>
-              if Pos.eqb sz_t sz_from && (sz_to <? sz_from)%positive
-              then Conv_Pure (@DVALUE_I sz_to (repr (unsigned i1)))
-              else Conv_Illegal "i-to-i ill-typed Trunc"
-
-          | DTYPE_I sz_t, DVALUE_Poison t, DTYPE_I sz_to =>
-              Conv_Pure (DVALUE_Poison t)
-
-          | _, _, _ => Conv_Illegal "ill-typed Trunc"
-          end
-
-      | Zext nneg => (* TODO: handle the nneg flag *)
-          match t1, x, t2 with
-          | DTYPE_I sz_t, @DVALUE_I sz_from i1, DTYPE_I sz_to =>
-              if Pos.eqb sz_t sz_from && (sz_from <? sz_to)%positive
-              then Conv_Pure (@DVALUE_I sz_to (repr (unsigned i1)))
-              else Conv_Illegal "i-to-i ill-typed Zext"
-
-          | DTYPE_I sz_t, DVALUE_Poison t, DTYPE_I sz_to =>
-              Conv_Pure (DVALUE_Poison t)
-
-          | _, _, _ => Conv_Illegal "ill-typed Zext"
-          end
-
-      | Sext =>
-          match t1, x, t2 with
-          | DTYPE_I sz_t, @DVALUE_I sz_from i1, DTYPE_I sz_to =>
-              if Pos.eqb sz_t sz_from && (sz_from <? sz_to)%positive
-              then Conv_Pure (@DVALUE_I sz_to (repr (signed i1)))
-              else Conv_Illegal "i-to-i ill-typed Sext"
-
-          | DTYPE_I sz_t, DVALUE_Poison t, DTYPE_I sz_to =>
-              Conv_Pure (DVALUE_Poison t)
-
-          | _, _, _ => Conv_Illegal "ill-typed Sext"
-          end
-
-      | Bitcast =>
-          if dtyp_eqb t1 t2
-          then Conv_Pure x
-          else if bit_sizeof_dtyp t1 =? bit_sizeof_dtyp t2
-               then
-                 let bytes := dvalue_to_dvalue_bytes x t1 in
-                 let dv_conv := ErrOOMPoison_handle_poison_and_oom DVALUE_Poison (@dvalue_bytes_to_dvalue ErrOOMPoison _ _ _ _ bytes t2) in
-                 match unIdent (unEitherT (unEitherT (unEitherT (unERR_UB_OOM dv_conv)))) with
-                 | inl (OOM_message oom) =>
-                     Conv_Oom ("Bitcast OOM: " ++ oom)
-                 | inr (inl (UB_message ub)) =>
-                     Conv_Illegal ("Bitcast UB: " ++ ub)
-                 | inr (inr (inl (ERR_message err))) =>
-                     Conv_Illegal ("Bitcast failure: " ++ err)
-                 | inr (inr (inr dv)) =>
-                     Conv_Pure dv
-                 end
-               else Conv_Illegal "unequal bitsize in cast"
-
-      | Uitofp nneg => (* TODO: handle the nneg flag *)
-          match t1, x, t2 with
-          | DTYPE_I sz_t, @DVALUE_I sz_from i1, DTYPE_FP FP_float =>
-              if Pos.eqb sz_t sz_from
-              then Conv_Pure (DVALUE_Float (Float32.of_intu (repr (unsigned i1))))
-              else Conv_Illegal "i-to-float ill-typed Uitofp"
-
-          | DTYPE_I sz_t, @DVALUE_I sz_from i1, DTYPE_FP FP_double =>
-              if Pos.eqb sz_t sz_from
-              then Conv_Pure (DVALUE_Double (Float.of_longu (repr (unsigned i1))))
-              else Conv_Illegal "i-to-double ill-typed Uitofp"
-
-          | DTYPE_I sz_t, DVALUE_Poison t, DTYPE_FP _ =>
-              Conv_Pure (DVALUE_Poison t)
-
-          | _, _, _ => Conv_Illegal "ill-typed Uitofp"
-          end
-
-      | Sitofp =>
-          match t1, x, t2 with
-          | DTYPE_I sz_t, @DVALUE_I sz_from i1, DTYPE_FP FP_float =>
-              if Pos.eqb sz_t sz_from
-              then Conv_Pure (DVALUE_Float (Float32.of_intu (repr (signed i1))))
-              else Conv_Illegal "i-to-float ill-typed Sitofp"
-
-          | DTYPE_I sz_t, @DVALUE_I sz_from i1, DTYPE_FP FP_double =>
-              if Pos.eqb sz_t sz_from
-              then Conv_Pure (DVALUE_Double (Float.of_longu (repr (signed i1))))
-              else Conv_Illegal "i-to-double ill-typed Sitofp"
-
-          | DTYPE_I sz_t, DVALUE_Poison t, DTYPE_FP _ =>
-              Conv_Pure (DVALUE_Poison t)
-
-          | _, _, _ => Conv_Illegal "ill-typed Sitofp"
-          end
-
-      | Inttoptr =>
-          match t1, t2 with
-          | DTYPE_I _, DTYPE_Pointer => Conv_ItoP x
-          | DTYPE_IPTR , DTYPE_Pointer => Conv_ItoP x
-          | _, _ => Conv_Illegal "Inttoptr got illegal arguments"
-          end
-      | Ptrtoint =>
-          match t1, t2 with
-          | DTYPE_Pointer, DTYPE_I _ => Conv_PtoI x
-          | DTYPE_Pointer, DTYPE_IPTR => Conv_PtoI x
-          | _, _ => Conv_Illegal "Ptrtoint got illegal arguments"
-          end
-
-      | Fptoui
-      | Fptosi
-      | Fptrunc _
-      | Fpext _
-      | Addrspacecast
-        => Conv_Illegal "TODO: unimplemented numeric conversion"
-      end.
-    Arguments get_conv_case _ _ _ _ : simpl nomatch.
-
-  End CONVERSIONS.
-
-  (* Variable ptr_size : nat. *)
-  (* Variable datalayout : DataLayout. *)
-  Definition ptr_size : nat := 8.
-
-  Definition addr := ADDR.addr.
-
-  Definition endianess : Endianess
-    := ENDIAN_LITTLE.
+  Definition addr := ADDR.addr.            
 
   (* Definition fp_alignment (bits : N) : option Alignment := *)
   (*   let fp_map := dl_floating_point_alignments datalayout *)
@@ -948,7 +777,7 @@ Module MakeBase (LP : LLVMParams) (MP : MEMORY_PARAMS LP) (Byte : ByteModule LP 
     Definition filter_uvalue_sid_matches (byte : uvalue) (uvs : list (N * uvalue)) : (list (N * uvalue) * list (N * uvalue))
       := filter_split (fun '(n, uv) => uvalue_sid_match byte uv) uvs.
 
-    (* TODO: satisfy termination checker *)
+
     Section Concretize.
       Context (M : Type -> Type).
       Context {HM : Monad M}.
@@ -958,491 +787,14 @@ Module MakeBase (LP : LLVMParams) (MP : MEMORY_PARAMS LP) (Byte : ByteModule LP 
       Context {ERR : RAISE_ERROR ERR_M}.
       Context {UB : RAISE_UB ERR_M}.
       Context {OOM : RAISE_OOM ERR_M}.
-      Variable lift_ue : forall {A}, ERR_M A -> M A.
-
-      Definition pre_concretized (acc : NMap (list (uvalue * dvalue))) (uv : uvalue) (sid : store_id) : option dvalue
-        := vs <- NM.find sid acc;;
-           assoc uv vs.
-
-      Definition new_concretized_byte
-        (acc : NMap (list (uvalue * dvalue))) (uv : uvalue) (dv : dvalue) (sid : store_id) : NMap (list (uvalue * dvalue))
-        := match NM.find sid acc with
-           | Some vs =>
-               match assoc uv vs with
-               | Some _ =>
-                   acc
-               | None =>
-                   NM.add sid (vs ++ [(uv, dv)]) acc
-               end
-           | None =>
-               NM.add sid [(uv, dv)] acc
-           end.
-
-      (* Take a UVALUE_ExtractByte, and replace the uvalue with a given dvalue...
-       *)
-      Definition uvalue_byte_replace_with_dvalue_byte (uv : uvalue) (dv : dvalue) : M dvalue_byte
-      := match uv with
-         | UVALUE_ExtractByte uv dt idx sid =>
-             ret (DVALUE_ExtractByte dv dt idx)
-         | _ => lift_ue (raise_error "uvalue_byte_replace_with_dvalue_byte called with non-UVALUE_ExtractByte value.")
-         end.
-
-      (* M will be err_or_ub / MPropT err_or_ub? *)
-      (* Define a sum type f a, g b.... a + b. Mutual recursive
-           function as one big function with sum type to select between
-           which "function" is being called *)
-      Fixpoint concretize_uvalueM (u : uvalue) : M dvalue :=
-        let
-          eval_select
-            (cnd : dvalue) (v1 v2 : uvalue) : M dvalue
-          := match cnd with
-             | DVALUE_Poison t =>
-                 (* TODO: Should be the type of the result of the select... *)
-                 ret (DVALUE_Poison t)
-             | @DVALUE_I 1 i =>
-                 if (@Integers.unsigned 1 i =? 1)%Z
-                 then concretize_uvalueM v1
-                 else concretize_uvalueM v2
-             | DVALUE_Vector _ conds =>
-                 let fix loop conds xs ys : M (list dvalue) :=
-                   match conds, xs, ys with
-                   | [], [], [] => ret []
-                   | (c::conds), (x::xs), (y::ys) =>
-                       selected <- match c with
-                                  | DVALUE_Poison t =>
-                                      (* TODO: Should be the type of the result of the select... *)
-                                      ret (DVALUE_Poison t)
-                                  | @DVALUE_I 1 i =>
-                                      if (@Integers.unsigned 1 i =? 1)%Z
-                                      then ret x
-                                      else ret y
-                                  | _ =>
-                                      lift_ue
-                                        (raise_error "concretize_uvalueM: ill-typed select, condition in vector was not poison or i1.")
-                                  end;;
-                       rest <- loop conds xs ys;;
-                       ret (selected :: rest)
-                   | _, _, _ =>
-                       lift_ue (raise_error "concretize_uvalueM: ill-typed vector select, length mismatch.")
-                   end in
-                 (* TODO: lazily concretize these vectors to avoid
-                   evaluating elements that aren't chosen? *)
-                 dv1 <- concretize_uvalueM v1;;
-                 dv2 <- concretize_uvalueM v2;;
-                 match dv1, dv2 with
-                 | DVALUE_Poison t, _ =>
-                     (* TODO: Should we make sure t is a vector type...? *)
-                     ret (DVALUE_Poison t)
-                 | DVALUE_Vector _ _, DVALUE_Poison t =>
-                     (* TODO: Should we make sure t is a vector type...? *)
-                     ret (DVALUE_Poison t)
-                 | DVALUE_Vector t xs, DVALUE_Vector _ ys =>
-                     selected <- loop conds xs ys;;
-                     ret (DVALUE_Vector t selected)
-                 | _, _ =>
-                     lift_ue (raise_error "concretize_uvalueM: ill-typed vector select, non-vector arguments")
-                 end
-             | _ => lift_ue (raise_error "concretize_uvalueM: ill-typed select.")
-             end
-        in
-      (* Concretize the uvalues in a list of UVALUE_ExtractBytes...
-
-       *)
-      (* Pick out uvalue bytes that are the same + have same sid
-
-         Concretize these identical uvalues...
-       *)
-      let fix concretize_uvalue_bytes_helper (acc : NMap (list (uvalue * dvalue))) (uvs : list uvalue) {struct uvs} : M (list dvalue_byte)
-      := match uvs with
-         | [] => ret []
-         | (uv::uvs) =>
-             match uv with
-             | UVALUE_ExtractByte byte_uv dt idx sid =>
-                 (* Check if this uvalue has been concretized already *)
-                 match pre_concretized acc byte_uv sid with
-                 | Some dv =>
-                     (* Use the pre_concretized value *)
-                     let dv_byte := DVALUE_ExtractByte dv dt idx in
-                     (* Concretize the rest of the bytes *)
-                     rest <- concretize_uvalue_bytes_helper acc uvs;;
-                     ret (dv_byte :: rest)
-                 | None =>
-                     (* Concretize the uvalue *)
-                     dv <- concretize_uvalueM byte_uv;;
-                     let dv_byte := DVALUE_ExtractByte dv dt idx in
-                     let acc := new_concretized_byte acc byte_uv dv sid in
-                     (* Concretize the rest of the bytes *)
-                     rest <- concretize_uvalue_bytes_helper acc uvs;;
-                     ret (dv_byte :: rest)
-                 end
-             | _ =>
-                 lift_ue (raise_error "concretize_uvalue_bytes_helper: non-byte in uvs.")
-             end
-         end in
-
-      let concretize_uvalue_bytes (uvs : list uvalue) : M (list dvalue_byte)
-      := concretize_uvalue_bytes_helper (@NM.empty _) uvs in
-
-      let extractbytes_to_dvalue (uvs : list uvalue) (dt : dtyp) : M dvalue
-      := dvbs <- concretize_uvalue_bytes uvs;;
-         lift_ue (ErrOOMPoison_handle_poison_and_oom DVALUE_Poison (dvalue_bytes_to_dvalue dvbs dt))
-      in
-      match u with
-        | UVALUE_Addr a                          => ret (DVALUE_Addr a)
-        | @UVALUE_I sz x                         => ret (@DVALUE_I sz x)
-        | UVALUE_IPTR x                          => ret (DVALUE_IPTR x)
-        | UVALUE_Double x                        => ret (DVALUE_Double x)
-        | UVALUE_Float x                         => ret (DVALUE_Float x)
-        | UVALUE_Undef t                         => undef_handler t
-        | UVALUE_Poison t                        => ret (DVALUE_Poison t)
-        | UVALUE_Oom t                           => ret (DVALUE_Oom t)
-        | UVALUE_None                            => ret DVALUE_None
-        | UVALUE_Struct fields                   => 'dfields <- map_monad concretize_uvalueM fields ;;
-                                                    ret (DVALUE_Struct dfields)
-        | UVALUE_Packed_struct fields            => 'dfields <- map_monad concretize_uvalueM fields ;;
-                                                    ret (DVALUE_Packed_struct dfields)
-        | UVALUE_Array t elts                    => 'delts <- map_monad concretize_uvalueM elts ;;
-                                                    ret (DVALUE_Array t delts)
-        | UVALUE_Vector t elts                   => 'delts <- map_monad concretize_uvalueM elts ;;
-                                                    ret (DVALUE_Vector t delts)
-        | UVALUE_IBinop iop v1 v2                => dv1 <- concretize_uvalueM v1 ;;
-                                                    dv2 <- concretize_uvalueM v2 ;;
-                                                    lift_ue (eval_iop iop dv1 dv2)
-        | UVALUE_ICmp ss cmp v1 v2                  => dv1 <- concretize_uvalueM v1 ;;
-                                                    dv2 <- concretize_uvalueM v2 ;;
-                                                    lift_ue (eval_icmp ss cmp dv1 dv2)
-        | UVALUE_FBinop fop fm v1 v2             => dv1 <- concretize_uvalueM v1 ;;
-                                                    dv2 <- concretize_uvalueM v2 ;;
-                                                    lift_ue (eval_fop fop dv1 dv2)
-        | UVALUE_Fneg fm t v                       => dv <- concretize_uvalueM v ;;
-                                                    lift_ue (eval_fneg dv)
-        | UVALUE_FCmp cmp v1 v2                  => dv1 <- concretize_uvalueM v1 ;;
-                                                    dv2 <- concretize_uvalueM v2 ;;
-                                                    lift_ue (eval_fcmp cmp dv1 dv2)
-
-        | UVALUE_Conversion conv t_from v t_to    =>
-            dv <- concretize_uvalueM v ;;
-            match get_conv_case conv t_from dv t_to with
-            | Conv_PtoI x =>
-                match x, t_to with
-                | DVALUE_Addr addr, DTYPE_I sz =>
-                    lift_ue (coerce_integer_to_int (Some sz) (ptr_to_int addr))
-                | DVALUE_Addr addr, DTYPE_IPTR =>
-                    lift_ue (coerce_integer_to_int None (ptr_to_int addr))
-                | _, _ =>
-                    lift_ue (raise_error "Invalid PTOI conversion")
-                end
-            | Conv_ItoP x =>
-                match int_to_ptr (dvalue_int_unsigned x) wildcard_prov with
-                | NoOom a =>
-                    ret (DVALUE_Addr a)
-                | Oom msg =>
-                    lift_ue (raise_oom ("concretize_uvalueM OOM in Conv_ItoP: " ++ msg))
-                end
-            | Conv_Pure x => ret x
-            | Conv_Oom s => lift_ue (raise_oom s)
-            | Conv_Illegal s => lift_ue (raise_error s)
-            end
-
-        | UVALUE_GetElementPtr t ua uvs =>
-            da <- concretize_uvalueM ua;;
-            dvs <- map_monad concretize_uvalueM uvs;;
-            match handle_gep t da dvs with
-            | inl err => lift_ue (raise_error err)
-            | inr (Oom msg) => lift_ue (raise_oom ("concretize_uvalueM OOM in GetElementPtr: " ++ msg))
-            | inr (NoOom dv) => ret dv
-            end
-        | UVALUE_ExtractValue t uv idxs =>
-            str <- concretize_uvalueM uv;;
-            let fix loop str idxs : ERR_M dvalue :=
-              match idxs with
-              | [] => ret str
-              | i :: tl =>
-                  v <- index_into_str_dv str i ;;
-                  loop v tl
-              end in
-            lift_ue (loop str idxs)
-
-        | UVALUE_Select cond v1 v2 =>
-            dcond <- concretize_uvalueM cond;;
-            eval_select dcond v1 v2
-
-        | UVALUE_ConcatBytes bytes dt =>
-            match N.eqb (N.of_nat (length bytes)) (sizeof_dtyp dt), all_extract_bytes_from_uvalue dt bytes with
-            | true, Some uv =>
-                match bytes with
-                | (UVALUE_ExtractByte uv _ _ _ :: _) => concretize_uvalueM uv
-                | _ => lift_ue (raise_error "ConcatBytes case... Should not happen.")
-                end
-            | _, _ => extractbytes_to_dvalue bytes dt
-            end
-
-        | UVALUE_ExtractByte byte dt idx sid =>
-            (* TODO: maybe this is just an error? ExtractByte should be guarded by ConcatBytes? *)
-            lift_ue (raise_error "Attempting to concretize UVALUE_ExtractByte, should not happen.")
-        | UVALUE_InsertValue t uv et elt idxs =>
-            str <- concretize_uvalueM uv;;
-            elt <- concretize_uvalueM elt;;
-            let fix loop str idxs : ERR_M dvalue :=
-              match idxs with
-              | [] => raise_error "Index was not provided"
-              | i :: nil =>
-                  v <- insert_into_str str elt i;;
-                  ret v
-              | i :: tl =>
-                      subfield <- index_into_str_dv str i;;
-                      modified_subfield <- loop subfield tl;;
-                      insert_into_str str modified_subfield i
-              end in
-            lift_ue (loop str idxs)
-        | UVALUE_ExtractElement vec_typ vec idx =>
-            dvec <- concretize_uvalueM vec;;
-            didx <- concretize_uvalueM idx;;
-            elt_typ <- match vec_typ with
-                       | DTYPE_Vector _ t => ret t
-                       | _ => lift_ue (raise_error "Invalid vector type for ExtractElement")
-                       end;;
-            lift_ue (index_into_vec_dv elt_typ dvec didx)
-        | UVALUE_InsertElement vec_typ vec elt idx =>
-            dvec <- concretize_uvalueM vec;;
-            didx <- concretize_uvalueM idx;;
-            delt <- concretize_uvalueM elt;;
-            lift_ue (insert_into_vec_dv vec_typ dvec delt didx)
-        | _ => lift_ue (raise_error ("concretize_uvalueM: Attempting to convert a partially non-reduced uvalue to dvalue. Should not happen: " ++ uvalue_constructor_string u))
-
-      end.
-
-      Lemma concretize_uvalueM_equation :
-        forall (u : uvalue),
-          concretize_uvalueM u =
-            let
-              eval_select
-                (cnd : dvalue) (v1 v2 : uvalue) : M dvalue
-              := match cnd with
-                 | DVALUE_Poison t =>
-                     (* TODO: Should be the type of the result of the select... *)
-                     ret (DVALUE_Poison t)
-                 | @DVALUE_I 1 i =>
-                     if (@Integers.unsigned 1 i =? 1)%Z
-                     then concretize_uvalueM v1
-                     else concretize_uvalueM v2
-                 | DVALUE_Vector _ conds =>
-                     let fix loop conds xs ys : M (list dvalue) :=
-                       match conds, xs, ys with
-                       | [], [], [] => ret []
-                       | (c::conds), (x::xs), (y::ys) =>
-                           selected <- match c with
-                                      | DVALUE_Poison t =>
-                                          (* TODO: Should be the type of the result of the select... *)
-                                          ret (DVALUE_Poison t)
-                                      | @DVALUE_I 1 i =>
-                                          if (@Integers.unsigned 1 i =? 1)%Z
-                                          then ret x
-                                          else ret y
-                                      | _ =>
-                                          lift_ue
-                                            (raise_error "concretize_uvalueM: ill-typed select, condition in vector was not poison or i1.")
-                                      end;;
-                           rest <- loop conds xs ys;;
-                           ret (selected :: rest)
-                       | _, _, _ =>
-                           lift_ue (raise_error "concretize_uvalueM: ill-typed vector select, length mismatch.")
-                       end in
-                     (* TODO: lazily concretize these vectors to avoid
-                   evaluating elements that aren't chosen? *)
-                     dv1 <- concretize_uvalueM v1;;
-                     dv2 <- concretize_uvalueM v2;;
-                     match dv1, dv2 with
-                     | DVALUE_Poison t, _ =>
-                         (* TODO: Should we make sure t is a vector type...? *)
-                         @ret M _ _ (DVALUE_Poison t)
-                     | DVALUE_Vector _ _, DVALUE_Poison t =>
-                         (* TODO: Should we make sure t is a vector type...? *)
-                         @ret M _ _ (DVALUE_Poison t)
-                     | DVALUE_Vector t xs, DVALUE_Vector _ ys =>
-                         selected <- loop conds xs ys;;
-                         @ret M _ _ (DVALUE_Vector t selected)
-                     | _, _ =>
-                         lift_ue (raise_error "concretize_uvalueM: ill-typed vector select, non-vector arguments")
-                     end
-                 | _ => lift_ue (raise_error "concretize_uvalueM: ill-typed select.")
-                 end
-            in
-            (* Concretize the uvalues in a list of UVALUE_ExtractBytes...
-
-             *)
-            (* Pick out uvalue bytes that are the same + have same sid
-
-         Concretize these identical uvalues...
-             *)
-            let fix concretize_uvalue_bytes_helper (acc : NMap (list (uvalue * dvalue))) (uvs : list uvalue) {struct uvs} : M (list dvalue_byte)
-              := match uvs with
-                 | [] => ret []
-                 | (uv::uvs) =>
-                     match uv with
-                     | UVALUE_ExtractByte byte_uv dt idx sid =>
-                         (* Check if this uvalue has been concretized already *)
-                         match pre_concretized acc byte_uv sid with
-                         | Some dv =>
-                             (* Use the pre_concretized value *)
-                             let dv_byte := DVALUE_ExtractByte dv dt idx in
-                             (* Concretize the rest of the bytes *)
-                             rest <- concretize_uvalue_bytes_helper acc uvs;;
-                             ret (dv_byte :: rest)
-                         | None =>
-                             (* Concretize the uvalue *)
-                             dv <- concretize_uvalueM byte_uv;;
-                             let dv_byte := DVALUE_ExtractByte dv dt idx in
-                             let acc := new_concretized_byte acc byte_uv dv sid in
-                             (* Concretize the rest of the bytes *)
-                             rest <- concretize_uvalue_bytes_helper acc uvs;;
-                             ret (dv_byte :: rest)
-                         end
-                     | _ =>
-                         lift_ue (raise_error "concretize_uvalue_bytes_helper: non-byte in uvs.")
-                     end
-                 end in
-
-            let concretize_uvalue_bytes (uvs : list uvalue) : M (list dvalue_byte)
-              := concretize_uvalue_bytes_helper (@NM.empty _) uvs in
-
-            let extractbytes_to_dvalue (uvs : list uvalue) (dt : dtyp) : M dvalue
-              := dvbs <- concretize_uvalue_bytes uvs;;
-                 lift_ue (ErrOOMPoison_handle_poison_and_oom DVALUE_Poison (dvalue_bytes_to_dvalue dvbs dt))
-            in
-            match u with
-            | UVALUE_Addr a                          => ret (DVALUE_Addr a)
-            | @UVALUE_I sz x                         => ret (@DVALUE_I sz x)
-            | UVALUE_IPTR x                          => ret (DVALUE_IPTR x)
-            | UVALUE_Double x                        => ret (DVALUE_Double x)
-            | UVALUE_Float x                         => ret (DVALUE_Float x)
-            | UVALUE_Undef t                         => undef_handler t
-            | UVALUE_Poison t                        => ret (DVALUE_Poison t)
-            | UVALUE_Oom t                           => ret (DVALUE_Oom t)
-            | UVALUE_None                            => ret DVALUE_None
-            | UVALUE_Struct fields                   => 'dfields <- map_monad (concretize_uvalueM) fields ;;
-                                                       ret (DVALUE_Struct dfields)
-            | UVALUE_Packed_struct fields            => 'dfields <- map_monad (concretize_uvalueM) fields ;;
-                                                       ret (DVALUE_Packed_struct dfields)
-            | UVALUE_Array t elts                    => 'delts <- map_monad (concretize_uvalueM) elts ;;
-                                                       ret (DVALUE_Array t delts)
-            | UVALUE_Vector t elts                   => 'delts <- map_monad (concretize_uvalueM) elts ;;
-                                                       ret (DVALUE_Vector t delts)
-            | UVALUE_IBinop iop v1 v2                => dv1 <- concretize_uvalueM v1 ;;
-                                                       dv2 <- concretize_uvalueM v2 ;;
-                                                       lift_ue (eval_iop iop dv1 dv2)
-            | UVALUE_ICmp ss cmp v1 v2                  => dv1 <- concretize_uvalueM v1 ;;
-                                                       dv2 <- concretize_uvalueM v2 ;;
-                                                       lift_ue (eval_icmp ss cmp dv1 dv2)
-            | UVALUE_FBinop fop fm v1 v2             => dv1 <- concretize_uvalueM v1 ;;
-                                                       dv2 <- concretize_uvalueM v2 ;;
-                                                       lift_ue (eval_fop fop dv1 dv2)
-            | UVALUE_Fneg fm t v                     => dv <- concretize_uvalueM v ;;
-                                                       lift_ue (eval_fneg dv)
-| UVALUE_FCmp cmp v1 v2                  => dv1 <- concretize_uvalueM v1 ;;
-                                                       dv2 <- concretize_uvalueM v2 ;;
-                                                       lift_ue (eval_fcmp cmp dv1 dv2)
-
-            | UVALUE_Conversion conv t_from v t_to    =>
-                dv <- concretize_uvalueM v ;;
-                match get_conv_case conv t_from dv t_to with
-                | Conv_PtoI x =>
-                    match x, t_to with
-                    | DVALUE_Addr addr, DTYPE_I sz =>
-                        lift_ue (coerce_integer_to_int (Some sz) (ptr_to_int addr))
-                    | DVALUE_Addr addr, DTYPE_IPTR =>
-                        lift_ue (coerce_integer_to_int None (ptr_to_int addr))
-                    | _, _ =>
-                        lift_ue (raise_error "Invalid PTOI conversion")
-                    end
-                | Conv_ItoP x =>
-                    match int_to_ptr (dvalue_int_unsigned x) wildcard_prov with
-                    | NoOom a =>
-                        ret (DVALUE_Addr a)
-                    | Oom msg =>
-                        lift_ue (raise_oom ("concretize_uvalueM OOM in Conv_ItoP: " ++ msg))
-                    end
-                | Conv_Pure x => ret x
-                | Conv_Oom s => lift_ue (raise_oom s)
-                | Conv_Illegal s => lift_ue (raise_error s)
-                end
-
-            | UVALUE_GetElementPtr t ua uvs =>
-                da <- concretize_uvalueM ua;;
-                dvs <- map_monad (concretize_uvalueM) uvs;;
-                match handle_gep t da dvs with
-                | inl err => lift_ue (raise_error err)
-                | inr (Oom msg) => lift_ue (raise_oom ("concretize_uvalueM OOM in GetElementPtr: " ++ msg))
-                | inr (NoOom dv) => ret dv
-                end
-            | UVALUE_ExtractValue t uv idxs =>
-                str <- concretize_uvalueM uv;;
-                let fix loop str idxs : ERR_M dvalue :=
-                  match idxs with
-                  | [] => ret str
-                  | i :: tl =>
-                      v <- index_into_str_dv str i ;;
-                      loop v tl
-                  end in
-                lift_ue (loop str idxs)
-
-            | UVALUE_Select cond v1 v2 =>
-                dcond <- concretize_uvalueM cond;;
-                eval_select dcond v1 v2
-
-            | UVALUE_ConcatBytes bytes dt =>
-                match N.eqb (N.of_nat (length bytes)) (sizeof_dtyp dt), Byte.all_extract_bytes_from_uvalue dt bytes with
-                | true, Some uv =>
-                    match bytes with
-                    | (UVALUE_ExtractByte uv _ _ _ :: _) => concretize_uvalueM uv
-                    | _ => lift_ue (raise_error "ConcatBytes case... Should not happen.")
-                    end
-                | _, _ => extractbytes_to_dvalue bytes dt
-                end
-
-            | UVALUE_ExtractByte byte dt idx sid =>
-                (* TODO: maybe this is just an error? ExtractByte should be guarded by ConcatBytes? *)
-                lift_ue (raise_error "Attempting to concretize UVALUE_ExtractByte, should not happen.")
-            | UVALUE_InsertValue t uv et elt idxs =>
-                str <- concretize_uvalueM uv;;
-                elt <- concretize_uvalueM elt;;
-                let fix loop str idxs : ERR_M dvalue :=
-                  match idxs with
-                  | [] => raise_error "Index was not provided"
-                  | i :: nil =>
-                      v <- insert_into_str str elt i;;
-                      ret v
-                  | i :: tl =>
-                      subfield <- index_into_str_dv str i;;
-                      modified_subfield <- loop subfield tl;;
-                      insert_into_str str modified_subfield i
-                  end in
-                lift_ue (loop str idxs)
-            | UVALUE_ExtractElement vec_typ vec idx =>
-                dvec <- concretize_uvalueM vec;;
-                didx <- concretize_uvalueM idx;;
-                elt_typ <- match vec_typ with
-                          | DTYPE_Vector _ t => ret t
-                          | _ => lift_ue (raise_error "Invalid vector type for ExtractElement")
-                          end;;
-                lift_ue (index_into_vec_dv elt_typ dvec didx)
-            | UVALUE_InsertElement vec_typ vec elt idx =>
-                dvec <- concretize_uvalueM vec;;
-                didx <- concretize_uvalueM idx;;
-                delt <- concretize_uvalueM elt;;
-                lift_ue (insert_into_vec_dv vec_typ dvec delt didx)
-            | _ => lift_ue (raise_error ("concretize_uvalueM: Attempting to convert a partially non-reduced uvalue to dvalue. Should not happen: " ++ uvalue_constructor_string u))
-            end.
-      Proof.
-        induction u; try reflexivity.
-      Qed.
+      Variable lift_ue : forall A, ERR_M A -> M A.
 
       Fixpoint concretize_uvalue_bytes_helper (acc : NMap (list (uvalue * dvalue))) (uvs : list uvalue) : M (list dvalue_byte)
       := match uvs with
          | [] => ret []
-         | (uv::uvs) =>
+         | (uv::uvs) => 
              match uv with
-             | UVALUE_ExtractByte byte_uv dt idx sid =>
+             | UVALUE_ExtractByte byte_uv dt idx sid => 
                  (* Check if this uvalue has been concretized already *)
                  match pre_concretized acc byte_uv sid with
                  | Some dv =>
@@ -1453,50 +805,52 @@ Module MakeBase (LP : LLVMParams) (MP : MEMORY_PARAMS LP) (Byte : ByteModule LP 
                      ret (dv_byte :: rest)
                  | None =>
                      (* Concretize the uvalue *)
-                     dv <- concretize_uvalueM byte_uv;;
+                     dv <- @concretize_uvalueM M HM undef_handler ERR_M HM_ERR ERR UB OOM lift_ue byte_uv;; 
                      let dv_byte := DVALUE_ExtractByte dv dt idx in
                      let acc := new_concretized_byte acc byte_uv dv sid in
                      (* Concretize the rest of the bytes *)
                      rest <- concretize_uvalue_bytes_helper acc uvs;;
                      ret (dv_byte :: rest)
-                 end
+                 end 
              | _ =>
-                 lift_ue (raise_error "concretize_uvalue_bytes_helper: non-byte in uvs.")
+                 lift_ue _ (raise_error "concretize_uvalue_bytes_helper: non-byte in uvs.")
              end
          end.
 
-      Lemma concretize_uvalue_bytes_helper_equation (acc : NMap (list (uvalue * dvalue))) (uvs : list uvalue) :
-        concretize_uvalue_bytes_helper acc uvs
-        = match uvs with
-           | [] => ret []
-           | (uv::uvs) =>
-               match uv with
-               | UVALUE_ExtractByte byte_uv dt idx sid =>
-                   (* Check if this uvalue has been concretized already *)
-                   match pre_concretized acc byte_uv sid with
-                   | Some dv =>
-                       (* Use the pre_concretized value *)
-                       let dv_byte := DVALUE_ExtractByte dv dt idx in
-                       (* Concretize the rest of the bytes *)
-                       rest <- concretize_uvalue_bytes_helper acc uvs;;
-                       ret (dv_byte :: rest)
-                   | None =>
-                       (* Concretize the uvalue *)
-                       dv <- concretize_uvalueM byte_uv;;
-                       let dv_byte := DVALUE_ExtractByte dv dt idx in
-                       let acc := new_concretized_byte acc byte_uv dv sid in
-                       (* Concretize the rest of the bytes *)
-                       rest <- concretize_uvalue_bytes_helper acc uvs;;
-                       ret (dv_byte :: rest)
-                   end
-               | _ =>
-                   lift_ue (raise_error "concretize_uvalue_bytes_helper: non-byte in uvs.")
-               end
-          end.
-      Proof.
-        induction uvs; try reflexivity.
-      Qed.
+      
+      (* Lemma concretize_uvalue_bytes_helper_equation (acc : NMap (list (uvalue * dvalue))) (uvs : list uvalue) : *)
+      (*   concretize_uvalue_bytes_helper acc uvs *)
+      (*   = match uvs with *)
+      (*      | [] => ret [] *)
+      (*      | (uv::uvs) => *)
+      (*          match uv with *)
+      (*          | UVALUE_ExtractByte byte_uv dt idx sid => *)
+      (*              (* Check if this uvalue has been concretized already *) *)
+      (*              match pre_concretized acc byte_uv sid with *)
+      (*              | Some dv => *)
+      (*                  (* Use the pre_concretized value *) *)
+      (*                  let dv_byte := DVALUE_ExtractByte dv dt idx in *)
+      (*                  (* Concretize the rest of the bytes *) *)
+      (*                  rest <- concretize_uvalue_bytes_helper acc uvs;; *)
+      (*                  ret (dv_byte :: rest) *)
+      (*              | None => *)
+      (*                  (* Concretize the uvalue *) *)
+      (*                  dv <- concretize_uvalueM byte_uv;; *)
+      (*                  let dv_byte := DVALUE_ExtractByte dv dt idx in *)
+      (*                  let acc := new_concretized_byte acc byte_uv dv sid in *)
+      (*                  (* Concretize the rest of the bytes *) *)
+      (*                  rest <- concretize_uvalue_bytes_helper acc uvs;; *)
+      (*                  ret (dv_byte :: rest) *)
+      (*              end *)
+      (*          | _ => *)
+      (*              lift_ue (raise_error "concretize_uvalue_bytes_helper: non-byte in uvs.") *)
+      (*          end *)
+      (*     end. *)
+      (* Proof. *)
+      (*   induction uvs; try reflexivity. *)
+      (* Qed. *)
 
+      (*
       Definition eval_select
         (cnd : dvalue) (v1 v2 : uvalue) : M dvalue
         := match cnd with
@@ -1603,7 +957,7 @@ Module MakeBase (LP : LLVMParams) (MP : MEMORY_PARAMS LP) (Byte : ByteModule LP 
       Proof.
         destruct cnd; try reflexivity.
       Qed.
-
+       *)
     End Concretize.
 
     Arguments concretize_uvalueM {_ _}.
